src/program_proof/tulip/program/txn/txn_delete.v
@@ -5,11 +5,12 @@ Section program.
   Context `{!heapGS Σ, !tulip_ghostG Σ}.
 
   Theorem wp_Txn__Delete txn tid key rds γ τ :
+    valid_key key ->
     {{{ own_txn txn tid rds γ τ ∗ (∃ vprev, txnmap_ptsto τ key vprev) }}}
       Txn__Delete #txn #(LitString key)
     {{{ RET #(); own_txn txn tid rds γ τ ∗ txnmap_ptsto τ key None }}}.
   Proof.
-    iIntros (Φ) "[Htxn [%v Hpt]] HΦ".
+    iIntros (Hvk Φ) "[Htxn [%v Hpt]] HΦ".
     wp_rec.
 
     (*@ func (txn *Txn) Delete(key string) {                                    @*)
@@ -21,6 +22,7 @@ Section program.
     iNamed "Htxn".
     wp_pures.
     wp_apply (wp_Txn__setwrs _ _ None with "Hwrs").
+    { apply Hvk. }
     iIntros "Hwrs".
     wp_pures.
     iApply "HΦ".
