src/program_proof/tulip/program/txn/txn_write.v
@@ -5,11 +5,12 @@ Section program.
   Context `{!heapGS Σ, !tulip_ghostG Σ}.
 
   Theorem wp_Txn__Write txn tid key value rds γ τ :
+    valid_key key ->
     {{{ own_txn txn tid rds γ τ ∗ (∃ vprev, txnmap_ptsto τ key vprev) }}}
       Txn__Write #txn #(LitString key) #(LitString value)
     {{{ RET #(); own_txn txn tid rds γ τ ∗ txnmap_ptsto τ key (Some value) }}}.
   Proof.
-    iIntros (Φ) "[Htxn [%v Hpt]] HΦ".
+    iIntros (Hvk Φ) "[Htxn [%v Hpt]] HΦ".
     wp_rec.
 
     (*@ func (txn *Txn) Write(key string, value string) {                       @*)
@@ -22,6 +23,7 @@ Section program.
     iNamed "Htxn".
     wp_pures.
     wp_apply (wp_Txn__setwrs _ _ (Some value) with "Hwrs").
+    { apply Hvk. }
     iIntros "Hwrs".
     wp_pures.
     iApply "HΦ".
